Source/IntegrationTests/TestFiles/LitTests/LitTest/lean/network.dfy
@@ -1,47 +1,69 @@
 // LIBRARY
-datatype Link = New(src: MachineID, dst: MachineID)
-datatype Channel = New(msgs: seq<Event>) {
+
+datatype Link = Link(src: MachineID, dst: MachineID)
+
+datatype Channel = Channel(msgs: seq<Event>) {
   predicate empty() {|msgs| == 0}
   predicate nonempty() {!empty()}
   predicate init() {empty()}
-  static function create(): Channel ensures create().init() { Channel.New(msgs := [])}
+  static function New(): Channel ensures New().init() { Channel(msgs := [])}
+
   function send(msg: Event): Channel {this.(msgs := msgs + [msg])}
   function receive(): (Event, Channel) requires nonempty() {(msgs[0], this.(msgs := msgs[1..]))}
   function drop(idx: nat): Channel {if idx < |msgs| then this.(msgs := msgs[..idx] + msgs[idx+1..]) else this}
 }
-datatype Network = New(channel: map<Link, Channel>) {
+
+datatype Network = Network(channel: map<Link, Channel>) {
   predicate init() {forall link <- channel :: channel[link].init()}
-  
+  static function New(): Network ensures New().init() {Network.Network(channel := map[])}
+
   predicate receivable (src: MachineID, dst: MachineID)
   {
-    var link := Link.New(src, dst);
+    var link := Link(src, dst);
     link in channel && channel[link].nonempty()
   }
+
   function ensure(link: Link): (res: Network)
     ensures link in res.channel
     ensures link in channel ==> res.channel[link] == channel[link]
     ensures link !in channel ==> res.channel[link].empty()
   {
-    if link in channel then this else this.(channel := channel[link := Channel.create()])
+    if link in channel then this else this.(channel := channel[link := Channel.New()])
   }
+
   function send(src: MachineID, msg: Event, dst: MachineID): Network
   {
-    var link := Link.New(src, dst);
+    var link := Link(src, dst);
     this.(channel := channel[link := ensure(link).channel[link].send(msg)])
   }
+
   function receive(src: MachineID, dst: MachineID): (Event, Network)
     requires receivable(src, dst)
   {
-    var link := Link.New(src, dst);
+    var link := Link(src, dst);
     var (msg, ch) := channel[link].receive();
     (msg, this.(channel := channel[link := ch]))
   }
+
   function peek (src: MachineID, dst: MachineID): Event
     requires receivable(src, dst)
   {
-    channel[Link.New(src, dst)].msgs[0]
+    channel[Link(src, dst)].msgs[0]
   }
-  function multicast(src: MachineID, event: Event, targets: set<MachineID>): Network
-  { this 
+
+  function multicast(src: MachineID, event: Event, targets: set<MachineID>): Network {
+    Network(
+      map link <- channel ::
+        if link.src == src && link.dst in targets then
+          Channel(channel[link].msgs + [event])
+        else
+          channel[link]
+    )
+  }
+
+  function multisend(src: MachineID, msgs: set<(MachineID, Event)>): Network {
+    if |msgs| == 0 then this else
+    var msg: (MachineID, Event) :| msg in  msgs;
+    this.send(src, msg.1, msg.0).multisend(src, msgs - {msg})
   }
 }
