Source/IntegrationTests/TestFiles/LitTests/LitTest/lean/Kermit2PC.dfy
@@ -4,63 +4,31 @@
 
 function time_speed(): nat
 {
-  var this_0 := 3;
-
-  this_0
+  3
 }
 
 function time_uncertainty(): nat
 {
-  var this_1 := 3;
-
-  this_1
+  3
 }
 
 function INVALID_TIME(): tTime
 {
-  var this_2 := 0 - 1;
-
-  this_2
+  0
 }
 
 function INVALID_VALUE(): tVal
 {
-  var this_3 := 0 - 1;
-
-  this_3
+  0
 }
 
-function key_shard(key: tKey, numShards: nat): nat
-{
-  var this_4 := key % numShards;
+function key_shard(key: tKey, numShards: nat): nat {0}
 
-  this_4
-}
+function max_time(t1: tTime, t2: tTime): tTime {0}
 
-function max_time(t1: tTime, t2: tTime): tTime
-{
-  var this_7 := if t1 <= t2 then
-                  var this_5 := t1;
-                  this_5 else
-                  var this_6 := t2;
-                  this_6;
+function value_of_key_at_time(versions: map<tKey, map<tTime, tVal>>, key: tKey, time: tTime): tVal {0}
 
-  this_7
-}
-
-function value_of_key_at_time(versions: map<tKey, map<tTime, tVal>>, key: tKey, time: tTime): tVal
-{
-  var this_8 := INVALID_VALUE();
-
-  this_8
-}
-
-function time_of_last_update(versions: map<tKey, map<tTime, tVal>>, key: tKey): tTime
-{
-  var this_9 := INVALID_TIME();
-
-  this_9
-}
+function time_of_last_update(versions: map<tKey, map<tTime, tVal>>, key: tKey): tTime {0}
 
 datatype MachineID = Clock(clock: ClockID) | Router(router: RouterID) | Shard(shard: ShardID)
 
@@ -70,7 +38,7 @@ datatype Message = New(target: MachineID, event: Event)
 
 datatype Machine = Clock(clock: Clock) | Router(router: Router) | Shard(shard: Shard)
 
-newtype tTime = nat
+type tTime = nat
 
 datatype tClockTime = New(earliest: tTime, latest: tTime)
 
@@ -152,13 +120,13 @@ datatype Clock = New(globaltime: nat, localtime: map<MachineID, tClockTime>, pen
 
 newtype RouterID = nat
 
-datatype RouterState = Init(entry: bool) | WaitForEvents(entry: bool) | Disconnected(entry: bool)
+datatype RouterState = Init(entry: bool) | EventLoop(entry: bool) | Disconnected(entry: bool) | Error(entry: bool)
 
 datatype Router = New(routerId: nat, localClock: MachineID, shards: map<nat, MachineID>, client: map<tTid, MachineID>, start_time: map<tTid, tTime>, participants: map<tTid, set<MachineID>>, lead_participant: map<tTid, MachineID>, committed: set<tTid>, prepare_responses: map<tTid, set<tShardPrepareRsp>>, prepare_commit_decision: map<tTid, bool>, prepare_commit_time: map<tTid, tTime>, state: RouterState)
 
 newtype ShardID = nat
 
-datatype ShardState = Init(entry: bool) | WaitForRequests(entry: bool)
+datatype ShardState = Init(entry: bool) | EventLoop(entry: bool) | Error(entry: bool)
 
 datatype Shard = New(shardId: nat, localClock: MachineID, clock: tTime, versions: map<tKey, map<tTime, tVal>>, write_buff: map<tTid, map<tKey, tVal>>, router: map<tTid, MachineID>, lead_shard: map<tTid, MachineID>, prepared: map<tTid, tTime>, committed: map<tTid, tTime>, aborted: set<tTid>, pending_reads: map<tShardReadReq, set<tTid>>, pending_updates: set<tShardUpdateReq>, locked_keys: set<tKey>, state: ShardState)
 
@@ -171,9 +139,12 @@ datatype System = New(machines: map<MachineID, Machine>, network: Network) {
     requires machines[dst].Clock?
     requires machines[dst].clock.state.EventLoop?
   {
-    var (event, network') := network.receive(src, dst);
+    var (event, network') :=
+      network.receive(src, dst);
 
-    var this_0 := this.(network := network');
+    var this_0 :=
+      this.(network :=
+      network');
 
     this_0
   }
@@ -187,9 +158,12 @@ datatype System = New(machines: map<MachineID, Machine>, network: Network) {
     requires machines[dst].Clock?
     requires machines[dst].clock.state.EventLoop?
   {
-    var (event, network') := network.receive(src, dst);
+    var (event, network') :=
+      network.receive(src, dst);
 
-    var this_0 := this.(network := network');
+    var this_0 :=
+      this.(network :=
+      network');
 
     this_0
   }
@@ -203,600 +177,1393 @@ datatype System = New(machines: map<MachineID, Machine>, network: Network) {
     requires machines[dst].Clock?
     requires machines[dst].clock.state.EventLoop?
   {
-    var (event, network') := network.receive(src, dst);
+    var (event, network') :=
+      network.receive(src, dst);
 
-    var this_0 := this.(network := network');
+    var this_0 :=
+      this.(network :=
+      network');
 
     this_0
   }
 
-  function deliver_eStartReq_to_Router_in_WaitForEvents(src: MachineID, dst: MachineID, payload: tStartReq): System
+  function deliver_eStartReq_to_Router_in_EventLoop(src: MachineID, dst: MachineID, payload: tStartReq): System
     requires src in machines
     requires dst in machines
     requires network.receivable(src, dst)
     requires network.receive(src, dst).0.eStartReq?
     requires network.receive(src, dst).0.TStartReq == payload
     requires machines[dst].Router?
-    requires machines[dst].router.state.WaitForEvents?
+    requires machines[dst].router.state.EventLoop?
   {
-    var (event, network') := network.receive(src, dst);
+    var (event, network') :=
+      network.receive(src, dst);
 
-    var this_2 := this.(network := network');
+    var this_2 :=
+      this.(network :=
+      network');
 
-    var this_1 := this_2.(machines := this_2.machines[dst := this_2.machines[dst].(router := this_2.machines[dst].router.(client := this_2.machines[dst].router.client[this_2.machines[dst].router.routerId * 1000 + |this_2.machines[dst].router.client| := payload.client]))]);
+    var tid: tTid :=
+      this_2.machines[dst].router.routerId * 1000 + |this_2.machines[dst].router.client|;
 
-    var this_0 := this_1.(network := this_1.network.send(dst, Event.eClockTimeReq(tClockTimeReq.New(dst, this_1.machines[dst].router.routerId * 1000 + |this_1.machines[dst].router.client|)), this_1.machines[dst].router.localClock));
+    var this_1 :=
+      this_2.(machines :=
+      this_2.machines[dst :=
+      this_2.machines[dst].(router :=
+      this_2.machines[dst].router.(client :=
+      this_2.machines[dst].router.client[tid :=
+      payload.client]))]);
+
+    var this_0 :=
+      this_1.(network :=
+      this_1.network.send(dst, Event.eClockTimeReq(tClockTimeReq.New(dst, tid)), this_1.machines[dst].router.localClock));
 
     this_0
   }
 
-  function deliver_eClockTimeRsp_to_Router_in_WaitForEvents(src: MachineID, dst: MachineID, clock: tClockTimeRsp): System
+  function deliver_eClockTimeRsp_to_Router_in_EventLoop(src: MachineID, dst: MachineID, clock: tClockTimeRsp): System
     requires src in machines
     requires dst in machines
     requires network.receivable(src, dst)
     requires network.receive(src, dst).0.eClockTimeRsp?
     requires network.receive(src, dst).0.TClockTimeRsp == clock
     requires machines[dst].Router?
-    requires machines[dst].router.state.WaitForEvents?
+    requires machines[dst].router.state.EventLoop?
   {
-    var (event, network') := network.receive(src, dst);
+    var (event, network') :=
+      network.receive(src, dst);
 
-    var this_3 := this.(network := network');
+    var this_5 :=
+      this.(network :=
+      network');
 
-    var this_2 := this_3.(machines := this_3.machines[dst := this_3.machines[dst].(router := this_3.machines[dst].router.(start_time := this_3.machines[dst].router.start_time[clock.requestId := clock.now.latest]))]);
+    var tid: tTid :=
+      clock.requestId;
 
-    var this_1 := this_2.(machines := this_2.machines[dst := this_2.machines[dst].(router := this_2.machines[dst].router.(participants := this_2.machines[dst].router.participants[clock.requestId := {}]))]);
+    var empty: set<MachineID> :=
+      {};
 
-    var this_0 := this_1.(network := this_1.network.send(dst, Event.eStartRsp(tStartRsp.New(dst, clock.requestId, this_1.machines[dst].router.start_time[clock.requestId])), this_1.machines[dst].router.client[clock.requestId]));
+    var this_4 :=
+      if
+        tid in this_5.machines[dst].router.client
+      then
+        var this_2 :=
+          this_5.(machines :=
+          this_5.machines[dst :=
+          this_5.machines[dst].(router :=
+          this_5.machines[dst].router.(start_time :=
+          this_5.machines[dst].router.start_time[tid :=
+          clock.now.latest]))]);
+        var this_1 :=
+          this_2.(machines :=
+          this_2.machines[dst :=
+          this_2.machines[dst].(router :=
+          this_2.machines[dst].router.(participants :=
+          this_2.machines[dst].router.participants[tid :=
+          empty]))]);
+        var this_0 :=
+          this_1.(network :=
+          this_1.network.send(dst, Event.eStartRsp(tStartRsp.New(dst, tid, this_1.machines[dst].router.start_time[tid])), this_1.machines[dst].router.client[tid]));
+        this_0
+      else
+        var this_3 :=
+          this_5.(machines :=
+          this_5.machines[dst :=
+          this_5.machines[dst].(router :=
+          this_5.machines[dst].router.(state :=
+          RouterState.Error(true)))]);
+        this_3;
 
-    this_0
+    this_4
   }
 
-  function deliver_eReadReq_to_Router_in_WaitForEvents(src: MachineID, dst: MachineID, read: tReadReq): System
+  function deliver_eReadReq_to_Router_in_EventLoop(src: MachineID, dst: MachineID, read: tReadReq): System
     requires src in machines
     requires dst in machines
     requires network.receivable(src, dst)
     requires network.receive(src, dst).0.eReadReq?
     requires network.receive(src, dst).0.TReadReq == read
     requires machines[dst].Router?
-    requires machines[dst].router.state.WaitForEvents?
+    requires machines[dst].router.state.EventLoop?
   {
-    var (event, network') := network.receive(src, dst);
+    var (event, network') :=
+      network.receive(src, dst);
 
-    var this_1 := this.(network := network');
+    var this_5 :=
+      this.(network :=
+      network');
 
-    var this_0 := this_1.(network := this_1.network.send(dst, Event.eShardReadReq(tShardReadReq.New(dst, read.tid, read.key, this_1.machines[dst].router.start_time[read.tid])), this_1.machines[dst].router.shards[key_shard(read.key, |this_1.machines[dst].router.shards|)]));
+    var this_4 :=
+      if
+        |this_5.machines[dst].router.shards| > 0
+      then
+        var sid: nat :=
+          key_shard(read.key, |this_5.machines[dst].router.shards|);
+        var this_2 :=
+          if
+            sid in this_5.machines[dst].router.shards && read.tid in this_5.machines[dst].router.start_time
+          then
+            var this_0 :=
+              this_5.(network :=
+              this_5.network.send(dst, Event.eShardReadReq(tShardReadReq.New(dst, read.tid, read.key, this_5.machines[dst].router.start_time[read.tid])), this_5.machines[dst].router.shards[sid]));
+            this_0
+          else
+            var this_1 :=
+              this_5.(machines :=
+              this_5.machines[dst :=
+              this_5.machines[dst].(router :=
+              this_5.machines[dst].router.(state :=
+              RouterState.Error(true)))]);
+            this_1;
+        this_2
+      else
+        var this_3 :=
+          this_5.(machines :=
+          this_5.machines[dst :=
+          this_5.machines[dst].(router :=
+          this_5.machines[dst].router.(state :=
+          RouterState.Error(true)))]);
+        this_3;
 
-    this_0
+    this_4
   }
 
-  function deliver_eShardReadRsp_to_Router_in_WaitForEvents(src: MachineID, dst: MachineID, read: tShardReadRsp): System
+  function deliver_eShardReadRsp_to_Router_in_EventLoop(src: MachineID, dst: MachineID, read: tShardReadRsp): System
     requires src in machines
     requires dst in machines
     requires network.receivable(src, dst)
     requires network.receive(src, dst).0.eShardReadRsp?
     requires network.receive(src, dst).0.TShardReadRsp == read
     requires machines[dst].Router?
-    requires machines[dst].router.state.WaitForEvents?
+    requires machines[dst].router.state.EventLoop?
   {
-    var (event, network') := network.receive(src, dst);
+    var (event, network') :=
+      network.receive(src, dst);
 
-    var this_4 := this.(network := network');
+    var this_6 :=
+      this.(network :=
+      network');
 
-    var this_3 := if read.status == tReqStatus.ABORT() then
-                    var this_1 := multicastAbort(dst, read.tid);
-                    var this_0 := this_1.(network := this_1.network.send(dst, Event.eReadRsp(tReadRsp.New(dst, read.tid, read.key, read.val, tReqStatus.ABORT())), this_1.machines[dst].router.client[read.tid]));
-                    this_0 else
-                    var this_2 := this_4.(network := this_4.network.send(dst, Event.eReadRsp(tReadRsp.New(dst, read.tid, read.key, read.val, tReqStatus.OK())), this_4.machines[dst].router.client[read.tid]));
-                    this_2;
+    var this_5 :=
+      if
+        read.tid in this_6.machines[dst].router.client
+      then
+        var this_3 :=
+          if
+            read.status == tReqStatus.ABORT()
+          then
+            var this_1 :=
+              this_6.multicastAbort(dst, read.tid);
+            var this_0 :=
+              this_1.(network :=
+              this_1.network.send(dst, Event.eReadRsp(tReadRsp.New(dst, read.tid, read.key, read.val, tReqStatus.ABORT())), this_1.machines[dst].router.client[read.tid]));
+            this_0
+          else
+            var this_2 :=
+              this_6.(network :=
+              this_6.network.send(dst, Event.eReadRsp(tReadRsp.New(dst, read.tid, read.key, read.val, tReqStatus.OK())), this_6.machines[dst].router.client[read.tid]));
+            this_2;
+        this_3
+      else
+        var this_4 :=
+          this_6.(machines :=
+          this_6.machines[dst :=
+          this_6.machines[dst].(router :=
+          this_6.machines[dst].router.(state :=
+          RouterState.Error(true)))]);
+        this_4;
 
-    this_3
+    this_5
   }
 
-  function deliver_eUpdateReq_to_Router_in_WaitForEvents(src: MachineID, dst: MachineID, update: tUpdateReq): System
+  function deliver_eUpdateReq_to_Router_in_EventLoop(src: MachineID, dst: MachineID, update: tUpdateReq): System
     requires src in machines
     requires dst in machines
     requires network.receivable(src, dst)
     requires network.receive(src, dst).0.eUpdateReq?
     requires network.receive(src, dst).0.TUpdateReq == update
     requires machines[dst].Router?
-    requires machines[dst].router.state.WaitForEvents?
+    requires machines[dst].router.state.EventLoop?
   {
-    var (event, network') := network.receive(src, dst);
+    var (event, network') :=
+      network.receive(src, dst);
 
-    var this_2 := this.(network := network');
+    var this_6 :=
+      this.(network :=
+      network');
 
-    var this_1 := this_2.(machines := this_2.machines[dst := this_2.machines[dst].(router := this_2.machines[dst].router.(participants := this_2.machines[dst].router.participants[update.tid := this_2.machines[dst].router.participants[update.tid] + {this_2.machines[dst].router.shards[key_shard(update.key, |this_2.machines[dst].router.shards|)]}]))]);
+    var this_5 :=
+      if
+        |this_6.machines[dst].router.shards| > 0
+      then
+        var sid: nat :=
+          key_shard(update.key, |this_6.machines[dst].router.shards|);
+        var this_3 :=
+          if
+            update.tid in this_6.machines[dst].router.participants && update.tid in this_6.machines[dst].router.start_time && sid in this_6.machines[dst].router.shards
+          then
+            var this_1 :=
+              this_6.(machines :=
+              this_6.machines[dst :=
+              this_6.machines[dst].(router :=
+              this_6.machines[dst].router.(participants :=
+              this_6.machines[dst].router.participants[update.tid :=
+              this_6.machines[dst].router.participants[update.tid] + {this_6.machines[dst].router.shards[sid]}]))]);
+            var this_0 :=
+              this_1.(network :=
+              this_1.network.send(dst, Event.eShardUpdateReq(tShardUpdateReq.New(dst, update.tid, update.key, update.val, this_1.machines[dst].router.start_time[update.tid])), this_1.machines[dst].router.shards[sid]));
+            this_0
+          else
+            var this_2 :=
+              this_6.(machines :=
+              this_6.machines[dst :=
+              this_6.machines[dst].(router :=
+              this_6.machines[dst].router.(state :=
+              RouterState.Error(true)))]);
+            this_2;
+        this_3
+      else
+        var this_4 :=
+          this_6.(machines :=
+          this_6.machines[dst :=
+          this_6.machines[dst].(router :=
+          this_6.machines[dst].router.(state :=
+          RouterState.Error(true)))]);
+        this_4;
 
-    var this_0 := this_1.(network := this_1.network.send(dst, Event.eShardUpdateReq(tShardUpdateReq.New(dst, update.tid, update.key, update.val, this_1.machines[dst].router.start_time[update.tid])), this_1.machines[dst].router.shards[key_shard(update.key, |this_1.machines[dst].router.shards|)]));
-
-    this_0
+    this_5
   }
 
-  function deliver_eShardUpdateRsp_to_Router_in_WaitForEvents(src: MachineID, dst: MachineID, update: tShardUpdateRsp): System
+  function deliver_eShardUpdateRsp_to_Router_in_EventLoop(src: MachineID, dst: MachineID, update: tShardUpdateRsp): System
     requires src in machines
     requires dst in machines
     requires network.receivable(src, dst)
     requires network.receive(src, dst).0.eShardUpdateRsp?
     requires network.receive(src, dst).0.TShardUpdateRsp == update
     requires machines[dst].Router?
-    requires machines[dst].router.state.WaitForEvents?
+    requires machines[dst].router.state.EventLoop?
   {
-    var (event, network') := network.receive(src, dst);
+    var (event, network') :=
+      network.receive(src, dst);
 
-    var this_4 := this.(network := network');
+    var this_6 :=
+      this.(network :=
+      network');
 
-    var this_3 := if update.status == tReqStatus.ABORT() then
-                    var this_1 := multicastAbort(dst, update.tid);
-                    var this_0 := this_1.(network := this_1.network.send(dst, Event.eUpdateRsp(tUpdateRsp.New(dst, update.tid, update.key, update.val, tReqStatus.ABORT())), this_1.machines[dst].router.client[update.tid]));
-                    this_0 else
-                    var this_2 := this_4.(network := this_4.network.send(dst, Event.eUpdateRsp(tUpdateRsp.New(dst, update.tid, update.key, update.val, tReqStatus.OK())), this_4.machines[dst].router.client[update.tid]));
-                    this_2;
+    var this_5 :=
+      if
+        update.tid in this_6.machines[dst].router.client
+      then
+        var this_3 :=
+          if
+            update.status == tReqStatus.ABORT()
+          then
+            var this_1 :=
+              this_6.multicastAbort(dst, update.tid);
+            var this_0 :=
+              this_1.(network :=
+              this_1.network.send(dst, Event.eUpdateRsp(tUpdateRsp.New(dst, update.tid, update.key, update.val, tReqStatus.ABORT())), this_1.machines[dst].router.client[update.tid]));
+            this_0
+          else
+            var this_2 :=
+              this_6.(network :=
+              this_6.network.send(dst, Event.eUpdateRsp(tUpdateRsp.New(dst, update.tid, update.key, update.val, tReqStatus.OK())), this_6.machines[dst].router.client[update.tid]));
+            this_2;
+        this_3
+      else
+        var this_4 :=
+          this_6.(machines :=
+          this_6.machines[dst :=
+          this_6.machines[dst].(router :=
+          this_6.machines[dst].router.(state :=
+          RouterState.Error(true)))]);
+        this_4;
 
-    this_3
+    this_5
   }
 
-  function deliver_eCommitReq_to_Router_in_WaitForEvents(src: MachineID, dst: MachineID, commit: tCommitReq, leader: MachineID): System
+  function deliver_eCommitReq_to_Router_in_EventLoop(src: MachineID, dst: MachineID, commit: tCommitReq, leader: MachineID): System
     requires src in machines
     requires dst in machines
     requires network.receivable(src, dst)
     requires network.receive(src, dst).0.eCommitReq?
     requires network.receive(src, dst).0.TCommitReq == commit
     requires machines[dst].Router?
-    requires machines[dst].router.state.WaitForEvents?
+    requires machines[dst].router.state.EventLoop?
     requires leader in this.machines[dst].router.shards.Values
   {
-    var (event, network') := network.receive(src, dst);
+    var (event, network') :=
+      network.receive(src, dst);
 
-    var this_6 := this.(network := network');
+    var this_8 :=
+      this.(network :=
+      network');
 
-    var this_5 := this_6;
+    var empty: set<tShardPrepareRsp> :=
+      {};
 
-    var this_4 := this_5.(machines := this_5.machines[dst := this_5.machines[dst].(router := this_5.machines[dst].router.(lead_participant := this_5.machines[dst].router.lead_participant[commit.tid := leader]))]);
+    var this_7 :=
+      this_8;
 
-    var this_3 := this_4.(machines := this_4.machines[dst := this_4.machines[dst].(router := this_4.machines[dst].router.(prepare_responses := this_4.machines[dst].router.prepare_responses[commit.tid := {}]))]);
+    var this_6 :=
+      if
+        commit.tid in this_7.machines[dst].router.start_time && commit.tid in this_7.machines[dst].router.participants
+      then
+        var this_4 :=
+          this_7.(machines :=
+          this_7.machines[dst :=
+          this_7.machines[dst].(router :=
+          this_7.machines[dst].router.(lead_participant :=
+          this_7.machines[dst].router.lead_participant[commit.tid :=
+          leader]))]);
+        var this_3 :=
+          this_4.(machines :=
+          this_4.machines[dst :=
+          this_4.machines[dst].(router :=
+          this_4.machines[dst].router.(prepare_responses :=
+          this_4.machines[dst].router.prepare_responses[commit.tid :=
+          empty]))]);
+        var this_2 :=
+          this_3.(machines :=
+          this_3.machines[dst :=
+          this_3.machines[dst].(router :=
+          this_3.machines[dst].router.(prepare_commit_decision :=
+          this_3.machines[dst].router.prepare_commit_decision[commit.tid :=
+          true]))]);
+        var this_1 :=
+          this_2.(machines :=
+          this_2.machines[dst :=
+          this_2.machines[dst].(router :=
+          this_2.machines[dst].router.(prepare_commit_time :=
+          this_2.machines[dst].router.prepare_commit_time[commit.tid :=
+          this_2.machines[dst].router.start_time[commit.tid]]))]);
+        var this_0 :=
+          this_1.(network :=
+          this_1.network.multisend(dst, set shard: MachineID | shard in this_1.machines[dst].router.participants[commit.tid] && true :: (shard, Event.eShardPrepareReq(tShardPrepareReq.New(dst, commit.tid, leader)))));
+        this_0
+      else
+        var this_5 :=
+          this_7.(machines :=
+          this_7.machines[dst :=
+          this_7.machines[dst].(router :=
+          this_7.machines[dst].router.(state :=
+          RouterState.Error(true)))]);
+        this_5;
 
-    var this_2 := this_3.(machines := this_3.machines[dst := this_3.machines[dst].(router := this_3.machines[dst].router.(prepare_commit_decision := this_3.machines[dst].router.prepare_commit_decision[commit.tid := true]))]);
-
-    var this_1 := this_2.(machines := this_2.machines[dst := this_2.machines[dst].(router := this_2.machines[dst].router.(prepare_commit_time := this_2.machines[dst].router.prepare_commit_time[commit.tid := this_2.machines[dst].router.start_time[commit.tid]]))]);
-
-    var this_0 := this_1.(network := this_1.network.multicast(dst, Event.eShardPrepareReq(tShardPrepareReq.New(dst, commit.tid, leader)), set shard: MachineID | shard in this_1.machines[dst].router.participants[commit.tid] && true :: shard));
-
-    this_0
+    this_6
   }
 
-  function deliver_eShardPrepareRsp_to_Router_in_WaitForEvents(src: MachineID, dst: MachineID, prepare: tShardPrepareRsp): System
+  function deliver_eShardPrepareRsp_to_Router_in_EventLoop(src: MachineID, dst: MachineID, prepare: tShardPrepareRsp): System
     requires src in machines
     requires dst in machines
     requires network.receivable(src, dst)
     requires network.receive(src, dst).0.eShardPrepareRsp?
     requires network.receive(src, dst).0.TShardPrepareRsp == prepare
     requires machines[dst].Router?
-    requires machines[dst].router.state.WaitForEvents?
+    requires machines[dst].router.state.EventLoop?
   {
-    var (event, network') := network.receive(src, dst);
+    var (event, network') :=
+      network.receive(src, dst);
 
-    var this_8 := this.(network := network');
+    var this_10 :=
+      this.(network :=
+      network');
 
-    var this_7 := this_8.(machines := this_8.machines[dst := this_8.machines[dst].(router := this_8.machines[dst].router.(prepare_responses := this_8.machines[dst].router.prepare_responses[prepare.tid := this_8.machines[dst].router.prepare_responses[prepare.tid] + {prepare}]))]);
+    var this_9 :=
+      if
+        prepare.tid in this_10.machines[dst].router.prepare_responses && prepare.tid in this_10.machines[dst].router.prepare_commit_decision && prepare.tid in this_10.machines[dst].router.prepare_commit_time && prepare.tid in this_10.machines[dst].router.participants && prepare.tid in this_10.machines[dst].router.lead_participant && prepare.tid in this_10.machines[dst].router.client
+      then
+        var this_7 :=
+          this_10.(machines :=
+          this_10.machines[dst :=
+          this_10.machines[dst].(router :=
+          this_10.machines[dst].router.(prepare_responses :=
+          this_10.machines[dst].router.prepare_responses[prepare.tid :=
+          this_10.machines[dst].router.prepare_responses[prepare.tid] + {prepare}]))]);
+        var this_6 :=
+          this_7.(machines :=
+          this_7.machines[dst :=
+          this_7.machines[dst].(router :=
+          this_7.machines[dst].router.(prepare_commit_decision :=
+          this_7.machines[dst].router.prepare_commit_decision[prepare.tid :=
+          this_7.machines[dst].router.prepare_commit_decision[prepare.tid] && prepare.status != tShardPrepareStatus.SHARD_ABORT()]))]);
+        var this_5 :=
+          this_6.(machines :=
+          this_6.machines[dst :=
+          this_6.machines[dst].(router :=
+          this_6.machines[dst].router.(prepare_commit_time :=
+          this_6.machines[dst].router.prepare_commit_time[prepare.tid :=
+          max_time(this_6.machines[dst].router.prepare_commit_time[prepare.tid], prepare.prepare_time)]))]);
+        var this_4 :=
+          if
+            |this_5.machines[dst].router.prepare_responses[prepare.tid]| == |this_5.machines[dst].router.participants[prepare.tid]|
+          then
+            var this_3 :=
+              if
+                this_5.machines[dst].router.prepare_commit_decision[prepare.tid]
+              then
+                var this_0 :=
+                  this_5.(network :=
+                  this_5.network.send(dst, Event.eShardCommitReq(tShardCommitReq.New(dst, prepare.tid, this_5.machines[dst].router.prepare_commit_time[prepare.tid], this_5.machines[dst].router.participants[prepare.tid])), this_5.machines[dst].router.lead_participant[prepare.tid]));
+                this_0
+              else
+                var this_2 :=
+                  this_5.multicastAbort(dst, prepare.tid);
+                var this_1 :=
+                  this_2.(network :=
+                  this_2.network.send(dst, Event.eCommitRsp(tCommitRsp.New(prepare.tid, tTxnStatus.ABORTED())), this_2.machines[dst].router.client[prepare.tid]));
+                this_1;
+            this_3
+          else
+            this_5;
+        this_4
+      else
+        var this_8 :=
+          this_10.(machines :=
+          this_10.machines[dst :=
+          this_10.machines[dst].(router :=
+          this_10.machines[dst].router.(state :=
+          RouterState.Error(true)))]);
+        this_8;
 
-    var this_6 := this_7.(machines := this_7.machines[dst := this_7.machines[dst].(router := this_7.machines[dst].router.(prepare_commit_decision := this_7.machines[dst].router.prepare_commit_decision[prepare.tid := this_7.machines[dst].router.prepare_commit_decision[prepare.tid] && prepare.status != tShardPrepareStatus.SHARD_ABORT()]))]);
-
-    var this_5 := this_6.(machines := this_6.machines[dst := this_6.machines[dst].(router := this_6.machines[dst].router.(prepare_commit_time := this_6.machines[dst].router.prepare_commit_time[prepare.tid := max_time(this_6.machines[dst].router.prepare_commit_time[prepare.tid], prepare.prepare_time)]))]);
-
-    var this_4 := if |this_5.machines[dst].router.prepare_responses[prepare.tid]| == |this_5.machines[dst].router.participants[prepare.tid]| then
-                    var this_3 := if this_5.machines[dst].router.prepare_commit_decision[prepare.tid] then
-                                    var this_0 := this_5.(network := this_5.network.send(dst, Event.eShardCommitReq(tShardCommitReq.New(dst, prepare.tid, this_5.machines[dst].router.prepare_commit_time[prepare.tid], this_5.machines[dst].router.participants[prepare.tid])), this_5.machines[dst].router.lead_participant[prepare.tid]));
-                                    this_0 else
-                                    var this_2 := multicastAbort(dst, prepare.tid);
-                                    var this_1 := this_2.(network := this_2.network.send(dst, Event.eCommitRsp(tCommitRsp.New(prepare.tid, tTxnStatus.ABORTED())), this_2.machines[dst].router.client[prepare.tid]));
-                                    this_1;
-                    this_3 else
-                    this_5;
-
-    this_4
+    this_9
   }
 
-  function deliver_eShardCommitRsp_to_Router_in_WaitForEvents(src: MachineID, dst: MachineID, commit: tShardCommitRsp): System
+  function deliver_eShardCommitRsp_to_Router_in_EventLoop(src: MachineID, dst: MachineID, commit: tShardCommitRsp): System
     requires src in machines
     requires dst in machines
     requires network.receivable(src, dst)
     requires network.receive(src, dst).0.eShardCommitRsp?
     requires network.receive(src, dst).0.TShardCommitRsp == commit
     requires machines[dst].Router?
-    requires machines[dst].router.state.WaitForEvents?
+    requires machines[dst].router.state.EventLoop?
   {
-    var (event, network') := network.receive(src, dst);
+    var (event, network') :=
+      network.receive(src, dst);
 
-    var this_8 := this.(network := network');
+    var this_10 :=
+      this.(network :=
+      network');
 
-    var this_7 := if commit.status == tTxnStatus.COMMITTED() then
-                    var this_3 := this_8;
-                    var this_2 := this_3.(machines := this_3.machines[dst := this_3.machines[dst].(router := this_3.machines[dst].router.(committed := this_3.machines[dst].router.committed + {commit.tid}))]);
-                    var this_1 := this_2.(network := this_2.network.multicast(dst, Event.eShardCommit(tShardCommit.New(commit.tid, commit.commit_time)), set shard: MachineID | shard in this_2.machines[dst].router.participants[commit.tid] && true :: shard));
-                    var this_0 := this_1.(network := this_1.network.send(dst, Event.eCommitRsp(tCommitRsp.New(commit.tid, tTxnStatus.COMMITTED())), this_1.machines[dst].router.client[commit.tid]));
-                    this_0 else
-                    var this_6 := this_8;
-                    var this_5 := multicastAbort(dst, commit.tid);
-                    var this_4 := this_5.(network := this_5.network.send(dst, Event.eCommitRsp(tCommitRsp.New(commit.tid, tTxnStatus.ABORTED())), this_5.machines[dst].router.client[commit.tid]));
-                    this_4;
+    var this_9 :=
+      if
+        commit.tid in this_10.machines[dst].router.participants && commit.tid in this_10.machines[dst].router.client
+      then
+        var this_7 :=
+          if
+            commit.status == tTxnStatus.COMMITTED()
+          then
+            var this_3 :=
+              this_10;
+            var this_2 :=
+              this_3.(machines :=
+              this_3.machines[dst :=
+              this_3.machines[dst].(router :=
+              this_3.machines[dst].router.(committed :=
+              this_3.machines[dst].router.committed + {commit.tid}))]);
+            var this_1 :=
+              this_2.(network :=
+              this_2.network.multisend(dst, set shard: MachineID | shard in this_2.machines[dst].router.participants[commit.tid] && true :: (shard, Event.eShardCommit(tShardCommit.New(commit.tid, commit.commit_time)))));
+            var this_0 :=
+              this_1.(network :=
+              this_1.network.send(dst, Event.eCommitRsp(tCommitRsp.New(commit.tid, tTxnStatus.COMMITTED())), this_1.machines[dst].router.client[commit.tid]));
+            this_0
+          else
+            var this_6 :=
+              this_10;
+            var this_5 :=
+              this_6.multicastAbort(dst, commit.tid);
+            var this_4 :=
+              this_5.(network :=
+              this_5.network.send(dst, Event.eCommitRsp(tCommitRsp.New(commit.tid, tTxnStatus.ABORTED())), this_5.machines[dst].router.client[commit.tid]));
+            this_4;
+        this_7
+      else
+        var this_8 :=
+          this_10.(machines :=
+          this_10.machines[dst :=
+          this_10.machines[dst].(router :=
+          this_10.machines[dst].router.(state :=
+          RouterState.Error(true)))]);
+        this_8;
 
-    this_7
+    this_9
   }
 
-  function deliver_eRollbackReq_to_Router_in_WaitForEvents(src: MachineID, dst: MachineID, rollback: tRollbackReq): System
+  function deliver_eRollbackReq_to_Router_in_EventLoop(src: MachineID, dst: MachineID, rollback: tRollbackReq): System
     requires src in machines
     requires dst in machines
     requires network.receivable(src, dst)
     requires network.receive(src, dst).0.eRollbackReq?
     requires network.receive(src, dst).0.TRollbackReq == rollback
     requires machines[dst].Router?
-    requires machines[dst].router.state.WaitForEvents?
+    requires machines[dst].router.state.EventLoop?
   {
-    var (event, network') := network.receive(src, dst);
+    var (event, network') :=
+      network.receive(src, dst);
 
-    var this_2 := this.(network := network');
+    var this_4 :=
+      this.(network :=
+      network');
 
-    var this_1 := multicastAbort(dst, rollback.tid);
+    var this_3 :=
+      if
+        rollback.tid in this_4.machines[dst].router.client
+      then
+        var this_1 :=
+          this_4.multicastAbort(dst, rollback.tid);
+        var this_0 :=
+          this_1.(network :=
+          this_1.network.send(dst, Event.eCommitRsp(tCommitRsp.New(rollback.tid, tTxnStatus.ABORTED())), this_1.machines[dst].router.client[rollback.tid]));
+        this_0
+      else
+        var this_2 :=
+          this_4.(machines :=
+          this_4.machines[dst :=
+          this_4.machines[dst].(router :=
+          this_4.machines[dst].router.(state :=
+          RouterState.Error(true)))]);
+        this_2;
 
-    var this_0 := this_1.(network := this_1.network.send(dst, Event.eCommitRsp(tCommitRsp.New(rollback.tid, tTxnStatus.ABORTED())), this_1.machines[dst].router.client[rollback.tid]));
-
-    this_0
+    this_3
   }
 
-  function deliver_eDisconnectRouter_to_Router_in_WaitForEvents(src: MachineID, dst: MachineID, disconnect: tDisconnectRouter): System
+  function deliver_eDisconnectRouter_to_Router_in_EventLoop(src: MachineID, dst: MachineID, disconnect: tDisconnectRouter): System
     requires src in machines
     requires dst in machines
     requires network.receivable(src, dst)
     requires network.receive(src, dst).0.eDisconnectRouter?
     requires network.receive(src, dst).0.TDisconnectRouter == disconnect
     requires machines[dst].Router?
-    requires machines[dst].router.state.WaitForEvents?
+    requires machines[dst].router.state.EventLoop?
   {
-    var (event, network') := network.receive(src, dst);
+    var (event, network') :=
+      network.receive(src, dst);
 
-    var this_2 := this.(network := network');
+    var this_2 :=
+      this.(network :=
+      network');
 
-    var this_1 := this_2.(network := this_2.network.send(dst, Event.eDisconnectRouterAck(tDisconnectRouterAck.New(dst)), disconnect.sender));
+    var this_1 :=
+      this_2.(network :=
+      this_2.network.send(dst, Event.eDisconnectRouterAck(tDisconnectRouterAck.New(dst)), disconnect.sender));
 
-    var this_0 := this_1.(machines := this_1.machines[dst := this_1.machines[dst].(router := this_1.machines[dst].router.(state := RouterState.Disconnected(true)))]);
+    var this_0 :=
+      this_1.(machines :=
+      this_1.machines[dst :=
+      this_1.machines[dst].(router :=
+      this_1.machines[dst].router.(state :=
+      RouterState.Disconnected(true)))]);
 
     this_0
   }
 
   function multicastAbort(dst: MachineID, tid: tTid): System
+    requires dst in machines
+    requires machines[dst].Router?
   {
-    var this_0 := this.(network := this.network.multicast(dst, Event.eShardAbort(tShardAbort.New(tid)), set shard: MachineID | shard in this.machines[dst].router.participants[tid] && true :: shard));
+    var this_3 :=
+      if
+        tid in this.machines[dst].router.participants
+      then
+        var this_1 :=
+          this;
+        var this_0 :=
+          this_1.(network :=
+          this_1.network.multisend(dst, set shard: MachineID | shard in this_1.machines[dst].router.participants[tid] && true :: (shard, Event.eShardAbort(tShardAbort.New(tid)))));
+        this_0
+      else
+        var this_2 :=
+          this.(machines :=
+          this.machines[dst :=
+          this.machines[dst].(router :=
+          this.machines[dst].router.(state :=
+          RouterState.Error(true)))]);
+        this_2;
 
-    this_0
+    this_3
   }
 
-  function deliver_eShardReadReq_to_Shard_in_WaitForRequests(src: MachineID, dst: MachineID, read: tShardReadReq): System
+  function deliver_eShardReadReq_to_Shard_in_EventLoop(src: MachineID, dst: MachineID, read: tShardReadReq): System
     requires src in machines
     requires dst in machines
     requires network.receivable(src, dst)
     requires network.receive(src, dst).0.eShardReadReq?
     requires network.receive(src, dst).0.TShardReadReq == read
     requires machines[dst].Shard?
-    requires machines[dst].shard.state.WaitForRequests?
+    requires machines[dst].shard.state.EventLoop?
   {
-    var (event, network') := network.receive(src, dst);
+    var (event, network') :=
+      network.receive(src, dst);
 
-    var this_9 := this.(network := network');
+    var this_12 :=
+      this.(network :=
+      network');
 
-    var this_8 := if read.tid in this_9.machines[dst].shard.aborted then
-                    var this_1 := this_9.(network := this_9.network.send(dst, Event.eShardReadRsp(tShardReadRsp.New(dst, read.tid, read.key, INVALID_VALUE(), tReqStatus.ABORT())), read.router));
-                    this_1 else
-                    var this_7 := if read.tid in this_9.machines[dst].shard.write_buff && read.key in this_9.machines[dst].shard.write_buff[read.tid] then
-                                    var this_2 := this_9.(network := this_9.network.send(dst, Event.eShardReadRsp(tShardReadRsp.New(dst, read.tid, read.key, this_9.machines[dst].shard.write_buff[read.tid][read.key], tReqStatus.OK())), read.router));
-                                    this_2 else
-                                    var this_6 := this_9.(machines := this_9.machines[dst := this_9.machines[dst].(shard := this_9.machines[dst].shard.(clock := max_time(this_9.machines[dst].shard.clock, read.start_time)))]);
-                                    var this_5 := this_6.(machines := this_6.machines[dst := this_6.machines[dst].(shard := this_6.machines[dst].shard.(pending_reads := this_6.machines[dst].shard.pending_reads[read := {}]))]);
-                                    var this_4 := this_5.(machines := this_5.machines[dst := this_5.machines[dst].(shard := this_5.machines[dst].shard.(pending_reads := this_5.machines[dst].shard.pending_reads[read := this_5.machines[dst].shard.pending_reads[read] + set tid: tTid | tid in this_5.machines[dst].shard.prepared && true && this_5.machines[dst].shard.prepared[tid] < read.start_time && tid in this_5.machines[dst].shard.write_buff && read.key in this_5.machines[dst].shard.write_buff[tid] :: tid]))]);
-                                    var this_3 := this_4;
-                                    this_3;
-                    this_7;
+    var empty: set<tTid> :=
+      {};
 
-    this_8
+    var this_11 :=
+      if
+        read.tid in this_12.machines[dst].shard.aborted
+      then
+        var this_4 :=
+          this_12.(network :=
+          this_12.network.send(dst, Event.eShardReadRsp(tShardReadRsp.New(dst, read.tid, read.key, INVALID_VALUE(), tReqStatus.ABORT())), read.router));
+        this_4
+      else
+        var this_10 :=
+          if
+            read.tid in this_12.machines[dst].shard.write_buff && read.key in this_12.machines[dst].shard.write_buff[read.tid]
+          then
+            var this_5 :=
+              this_12.(network :=
+              this_12.network.send(dst, Event.eShardReadRsp(tShardReadRsp.New(dst, read.tid, read.key, this_12.machines[dst].shard.write_buff[read.tid][read.key], tReqStatus.OK())), read.router));
+            this_5
+          else
+            var this_9 :=
+              this_12.(machines :=
+              this_12.machines[dst :=
+              this_12.machines[dst].(shard :=
+              this_12.machines[dst].shard.(clock :=
+              max_time(this_12.machines[dst].shard.clock, read.start_time)))]);
+            var this_8 :=
+              this_9.(machines :=
+              this_9.machines[dst :=
+              this_9.machines[dst].(shard :=
+              this_9.machines[dst].shard.(pending_reads :=
+              this_9.machines[dst].shard.pending_reads[read :=
+              empty]))]);
+            var this_7 :=
+              this_8.(machines :=
+              this_8.machines[dst :=
+              this_8.machines[dst].(shard :=
+              this_8.machines[dst].shard.(pending_reads :=
+              this_8.machines[dst].shard.pending_reads[read :=
+              this_8.machines[dst].shard.pending_reads[read] + set tid: tTid | tid in this_8.machines[dst].shard.prepared && true && this_8.machines[dst].shard.prepared[tid] < read.start_time && tid in this_8.machines[dst].shard.write_buff && read.key in this_8.machines[dst].shard.write_buff[tid] :: tid]))]);
+            var this_6 :=
+              this_7.(network :=
+              this_7.network.multisend(dst, set tid: tTid | tid in this_7.machines[dst].shard.pending_reads[read] && true && tid in this_7.machines[dst].shard.lead_shard :: (this_7.machines[dst].shard.lead_shard[tid], Event.eShardInquireReq(tShardInquireReq.New(dst, tid, read)))));
+            this_6;
+        this_10;
+
+    this_11
   }
 
-  function deliver_eShardInquireRsp_to_Shard_in_WaitForRequests(src: MachineID, dst: MachineID, inquire: tShardInquireRsp): System
+  function deliver_eShardInquireRsp_to_Shard_in_EventLoop(src: MachineID, dst: MachineID, inquire: tShardInquireRsp): System
     requires src in machines
     requires dst in machines
     requires network.receivable(src, dst)
     requires network.receive(src, dst).0.eShardInquireRsp?
     requires network.receive(src, dst).0.TShardInquireRsp == inquire
     requires machines[dst].Shard?
-    requires machines[dst].shard.state.WaitForRequests?
+    requires machines[dst].shard.state.EventLoop?
   {
-    var (event, network') := network.receive(src, dst);
+    var (event, network') :=
+      network.receive(src, dst);
 
-    var this_3 := this.(network := network');
+    var this_4 :=
+      this.(network :=
+      network');
 
-    var this_2 := if inquire.read in this_3.machines[dst].shard.pending_reads && inquire.tid in this_3.machines[dst].shard.pending_reads[inquire.read] then
-                    var this_1 := if !(inquire.status == tTxnStatus.COMMITTED() && inquire.commit_time < inquire.read.start_time) then
-                                    var this_0 := this_3.(machines := this_3.machines[dst := this_3.machines[dst].(shard := this_3.machines[dst].shard.(pending_reads := this_3.machines[dst].shard.pending_reads[inquire.read := this_3.machines[dst].shard.pending_reads[inquire.read] - {inquire.tid}]))]);
-                                    this_0 else
-                                    this_3;
-                    this_1 else
-                    this_3;
+    var this_3 :=
+      if
+        inquire.read in this_4.machines[dst].shard.pending_reads && inquire.tid in this_4.machines[dst].shard.pending_reads[inquire.read]
+      then
+        var this_1 :=
+          if
+            !(inquire.status == tTxnStatus.COMMITTED() && inquire.commit_time < inquire.read.start_time)
+          then
+            var this_0 :=
+              this_4.(machines :=
+              this_4.machines[dst :=
+              this_4.machines[dst].(shard :=
+              this_4.machines[dst].shard.(pending_reads :=
+              this_4.machines[dst].shard.pending_reads[inquire.read :=
+              this_4.machines[dst].shard.pending_reads[inquire.read] - {inquire.tid}]))]);
+            this_0
+          else
+            this_4;
+        this_1
+      else
+        var this_2 :=
+          this_4.(machines :=
+          this_4.machines[dst :=
+          this_4.machines[dst].(shard :=
+          this_4.machines[dst].shard.(state :=
+          ShardState.Error(true)))]);
+        this_2;
 
-    this_2
+    this_3
   }
 
-  function deliver_eTriggerReadRsp_to_Shard_in_WaitForRequests(src: MachineID, dst: MachineID, read: tShardReadReq): System
+  function deliver_eTriggerReadRsp_to_Shard_in_EventLoop(src: MachineID, dst: MachineID, read: tShardReadReq): System
     requires src in machines
     requires dst in machines
     requires network.receivable(src, dst)
     requires network.receive(src, dst).0.eTriggerReadRsp?
     requires machines[dst].Shard?
-    requires machines[dst].shard.state.WaitForRequests?
+    requires machines[dst].shard.state.EventLoop?
     requires read in this.machines[dst].shard.pending_reads
   {
-    var (event, network') := network.receive(src, dst);
+    var (event, network') :=
+      network.receive(src, dst);
 
-    var this_5 := this.(network := network');
+    var this_5 :=
+      this.(network :=
+      network');
 
-    var this_4 := if |this_5.machines[dst].shard.pending_reads| > 0 then
-                    var this_3 := this_5;
-                    var this_2 := if |this_3.machines[dst].shard.pending_reads[read]| == 0 then
-                                    var this_1 := this_3.(machines := this_3.machines[dst := this_3.machines[dst].(shard := this_3.machines[dst].shard.(pending_reads := this_3.machines[dst].shard.pending_reads - {read}))]);
-                                    var this_0 := this_1.(network := this_1.network.send(dst, Event.eShardReadRsp(tShardReadRsp.New(dst, read.tid, read.key, value_of_key_at_time(this_1.machines[dst].shard.versions, read.key, read.start_time), tReqStatus.OK())), read.router));
-                                    this_0 else
-                                    this_3;
-                    this_2 else
-                    this_5;
+    var this_4 :=
+      if
+        |this_5.machines[dst].shard.pending_reads| > 0
+      then
+        var this_3 :=
+          this_5;
+        var this_2 :=
+          if
+            |this_3.machines[dst].shard.pending_reads[read]| == 0
+          then
+            var this_1 :=
+              this_3.(machines :=
+              this_3.machines[dst :=
+              this_3.machines[dst].(shard :=
+              this_3.machines[dst].shard.(pending_reads :=
+              this_3.machines[dst].shard.pending_reads - {read}))]);
+            var val: tVal :=
+              value_of_key_at_time(this_1.machines[dst].shard.versions, read.key, read.start_time);
+            var this_0 :=
+              this_1.(network :=
+              this_1.network.send(dst, Event.eShardReadRsp(tShardReadRsp.New(dst, read.tid, read.key, val, tReqStatus.OK())), read.router));
+            this_0
+          else
+            this_3;
+        this_2
+      else
+        this_5;
 
     this_4
   }
 
-  function deliver_eShardUpdateReq_to_Shard_in_WaitForRequests(src: MachineID, dst: MachineID, update: tShardUpdateReq): System
+  function deliver_eShardUpdateReq_to_Shard_in_EventLoop(src: MachineID, dst: MachineID, update: tShardUpdateReq): System
     requires src in machines
     requires dst in machines
     requires network.receivable(src, dst)
     requires network.receive(src, dst).0.eShardUpdateReq?
     requires network.receive(src, dst).0.TShardUpdateReq == update
     requires machines[dst].Shard?
-    requires machines[dst].shard.state.WaitForRequests?
+    requires machines[dst].shard.state.EventLoop?
   {
-    var (event, network') := network.receive(src, dst);
+    var (event, network') :=
+      network.receive(src, dst);
 
-    var this_6 := this.(network := network');
+    var this_6 :=
+      this.(network :=
+      network');
 
-    var this_5 := if update.tid in this_6.machines[dst].shard.aborted then
-                    var this_0 := this_6.(network := this_6.network.send(dst, Event.eShardUpdateRsp(tShardUpdateRsp.New(dst, update.tid, update.key, update.val, tReqStatus.ABORT())), update.router));
-                    this_0 else
-                    var this_4 := if update.tid in this_6.machines[dst].shard.write_buff && update.key in this_6.machines[dst].shard.write_buff[update.tid] then
-                                    var this_2 := this_6.(machines := this_6.machines[dst := this_6.machines[dst].(shard := this_6.machines[dst].shard.(write_buff := this_6.machines[dst].shard.write_buff[update.tid := this_6.machines[dst].shard.write_buff[update.tid][update.key := update.val]]))]);
-                                    var this_1 := this_2.(network := this_2.network.send(dst, Event.eShardUpdateRsp(tShardUpdateRsp.New(dst, update.tid, update.key, update.val, tReqStatus.OK())), update.router));
-                                    this_1 else
-                                    var this_3 := this_6.(machines := this_6.machines[dst := this_6.machines[dst].(shard := this_6.machines[dst].shard.(pending_updates := this_6.machines[dst].shard.pending_updates + {update}))]);
-                                    this_3;
-                    this_4;
+    var this_5 :=
+      if
+        update.tid in this_6.machines[dst].shard.aborted
+      then
+        var this_0 :=
+          this_6.(network :=
+          this_6.network.send(dst, Event.eShardUpdateRsp(tShardUpdateRsp.New(dst, update.tid, update.key, update.val, tReqStatus.ABORT())), update.router));
+        this_0
+      else
+        var this_4 :=
+          if
+            update.tid in this_6.machines[dst].shard.write_buff && update.key in this_6.machines[dst].shard.write_buff[update.tid]
+          then
+            var this_2 :=
+              this_6.(machines :=
+              this_6.machines[dst :=
+              this_6.machines[dst].(shard :=
+              this_6.machines[dst].shard.(write_buff :=
+              this_6.machines[dst].shard.write_buff[update.tid :=
+              this_6.machines[dst].shard.write_buff[update.tid][update.key :=
+              update.val]]))]);
+            var this_1 :=
+              this_2.(network :=
+              this_2.network.send(dst, Event.eShardUpdateRsp(tShardUpdateRsp.New(dst, update.tid, update.key, update.val, tReqStatus.OK())), update.router));
+            this_1
+          else
+            var this_3 :=
+              this_6.(machines :=
+              this_6.machines[dst :=
+              this_6.machines[dst].(shard :=
+              this_6.machines[dst].shard.(pending_updates :=
+              this_6.machines[dst].shard.pending_updates + {update}))]);
+            this_3;
+        this_4;
 
     this_5
   }
 
-  function deliver_eTriggerUpdateRsp_to_Shard_in_WaitForRequests(src: MachineID, dst: MachineID, update: tShardUpdateReq): System
+  function deliver_eTriggerUpdateRsp_to_Shard_in_EventLoop(src: MachineID, dst: MachineID, update: tShardUpdateReq): System
     requires src in machines
     requires dst in machines
     requires network.receivable(src, dst)
     requires network.receive(src, dst).0.eTriggerUpdateRsp?
     requires machines[dst].Shard?
-    requires machines[dst].shard.state.WaitForRequests?
+    requires machines[dst].shard.state.EventLoop?
     requires update in this.machines[dst].shard.pending_updates
   {
-    var (event, network') := network.receive(src, dst);
+    var (event, network') :=
+      network.receive(src, dst);
 
-    var this_13 := this.(network := network');
+    var this_13 :=
+      this.(network :=
+      network');
 
-    var this_12 := if |this_13.machines[dst].shard.pending_updates| > 0 then
-                     var this_11 := this_13;
-                     var this_10 := if !(update.key in this_11.machines[dst].shard.locked_keys) then
-                                      var this_9 := this_11.(machines := this_11.machines[dst := this_11.machines[dst].(shard := this_11.machines[dst].shard.(locked_keys := this_11.machines[dst].shard.locked_keys + {update.key}))]);
-                                      var this_8 := if !(update.tid in this_9.machines[dst].shard.write_buff) then
-                                                      var this_7 := this_9.(machines := this_9.machines[dst := this_9.machines[dst].(shard := this_9.machines[dst].shard.(write_buff := this_9.machines[dst].shard.write_buff[update.tid := map[]]))]);
-                                                      this_7 else
-                                                      this_9;
-                                      var this_6 := if time_of_last_update(this_8.machines[dst].shard.versions, update.key) < update.start_time then
-                                                      var this_1 := this_8.(machines := this_8.machines[dst := this_8.machines[dst].(shard := this_8.machines[dst].shard.(write_buff := this_8.machines[dst].shard.write_buff[update.tid := this_8.machines[dst].shard.write_buff[update.tid][update.key := update.val]]))]);
-                                                      var this_0 := this_1.(network := this_1.network.send(dst, Event.eShardUpdateRsp(tShardUpdateRsp.New(dst, update.tid, update.key, update.val, tReqStatus.OK())), update.router));
-                                                      this_0 else
-                                                      var this_5 := this_8.(machines := this_8.machines[dst := this_8.machines[dst].(shard := this_8.machines[dst].shard.(locked_keys := this_8.machines[dst].shard.locked_keys - set key: tKey | key in this_8.machines[dst].shard.write_buff[update.tid] && true :: key))]);
-                                                      var this_4 := this_5.(machines := this_5.machines[dst := this_5.machines[dst].(shard := this_5.machines[dst].shard.(write_buff := this_5.machines[dst].shard.write_buff - {update.tid}))]);
-                                                      var this_3 := this_4.(machines := this_4.machines[dst := this_4.machines[dst].(shard := this_4.machines[dst].shard.(aborted := this_4.machines[dst].shard.aborted + {update.tid}))]);
-                                                      var this_2 := this_3.(network := this_3.network.send(dst, Event.eShardUpdateRsp(tShardUpdateRsp.New(dst, update.tid, update.key, update.val, tReqStatus.ABORT())), update.router));
-                                                      this_2;
-                                      this_6 else
-                                      this_11;
-                     this_10 else
-                     this_13;
+    var empty: map<tKey, tVal> :=
+      map[];
+
+    var this_12 :=
+      if
+        |this_13.machines[dst].shard.pending_updates| > 0
+      then
+        var this_11 :=
+          this_13;
+        var this_10 :=
+          if
+            !(update.key in this_11.machines[dst].shard.locked_keys)
+          then
+            var this_9 :=
+              this_11.(machines :=
+              this_11.machines[dst :=
+              this_11.machines[dst].(shard :=
+              this_11.machines[dst].shard.(locked_keys :=
+              this_11.machines[dst].shard.locked_keys + {update.key}))]);
+            var this_8 :=
+              if
+                !(update.tid in this_9.machines[dst].shard.write_buff)
+              then
+                var this_7 :=
+                  this_9.(machines :=
+                  this_9.machines[dst :=
+                  this_9.machines[dst].(shard :=
+                  this_9.machines[dst].shard.(write_buff :=
+                  this_9.machines[dst].shard.write_buff[update.tid :=
+                  empty]))]);
+                this_7
+              else
+                this_9;
+            var this_6 :=
+              if
+                time_of_last_update(this_8.machines[dst].shard.versions, update.key) < update.start_time
+              then
+                var this_1 :=
+                  this_8.(machines :=
+                  this_8.machines[dst :=
+                  this_8.machines[dst].(shard :=
+                  this_8.machines[dst].shard.(write_buff :=
+                  this_8.machines[dst].shard.write_buff[update.tid :=
+                  this_8.machines[dst].shard.write_buff[update.tid][update.key :=
+                  update.val]]))]);
+                var this_0 :=
+                  this_1.(network :=
+                  this_1.network.send(dst, Event.eShardUpdateRsp(tShardUpdateRsp.New(dst, update.tid, update.key, update.val, tReqStatus.OK())), update.router));
+                this_0
+              else
+                var this_5 :=
+                  this_8.(machines :=
+                  this_8.machines[dst :=
+                  this_8.machines[dst].(shard :=
+                  this_8.machines[dst].shard.(locked_keys :=
+                  this_8.machines[dst].shard.locked_keys - set key: tKey | key in this_8.machines[dst].shard.write_buff[update.tid] && true :: key))]);
+                var this_4 :=
+                  this_5.(machines :=
+                  this_5.machines[dst :=
+                  this_5.machines[dst].(shard :=
+                  this_5.machines[dst].shard.(write_buff :=
+                  this_5.machines[dst].shard.write_buff - {update.tid}))]);
+                var this_3 :=
+                  this_4.(machines :=
+                  this_4.machines[dst :=
+                  this_4.machines[dst].(shard :=
+                  this_4.machines[dst].shard.(aborted :=
+                  this_4.machines[dst].shard.aborted + {update.tid}))]);
+                var this_2 :=
+                  this_3.(network :=
+                  this_3.network.send(dst, Event.eShardUpdateRsp(tShardUpdateRsp.New(dst, update.tid, update.key, update.val, tReqStatus.ABORT())), update.router));
+                this_2;
+            this_6
+          else
+            this_11;
+        this_10
+      else
+        this_13;
 
     this_12
   }
 
-  function deliver_eShardPrepareReq_to_Shard_in_WaitForRequests(src: MachineID, dst: MachineID, prepare: tShardPrepareReq): System
+  function deliver_eShardPrepareReq_to_Shard_in_EventLoop(src: MachineID, dst: MachineID, prepare: tShardPrepareReq): System
     requires src in machines
     requires dst in machines
     requires network.receivable(src, dst)
     requires network.receive(src, dst).0.eShardPrepareReq?
     requires network.receive(src, dst).0.TShardPrepareReq == prepare
     requires machines[dst].Shard?
-    requires machines[dst].shard.state.WaitForRequests?
+    requires machines[dst].shard.state.EventLoop?
   {
-    var (event, network') := network.receive(src, dst);
+    var (event, network') :=
+      network.receive(src, dst);
 
-    var this_5 := this.(network := network');
+    var this_5 :=
+      this.(network :=
+      network');
 
-    var this_4 := if prepare.tid in this_5.machines[dst].shard.aborted then
-                    var this_0 := this_5.(network := this_5.network.send(dst, Event.eShardPrepareRsp(tShardPrepareRsp.New(dst, prepare.tid, tShardPrepareStatus.SHARD_ABORT(), INVALID_TIME())), prepare.router));
-                    this_0 else
-                    var this_3 := this_5.(machines := this_5.machines[dst := this_5.machines[dst].(shard := this_5.machines[dst].shard.(router := this_5.machines[dst].shard.router[prepare.tid := prepare.router]))]);
-                    var this_2 := this_3.(machines := this_3.machines[dst := this_3.machines[dst].(shard := this_3.machines[dst].shard.(lead_shard := this_3.machines[dst].shard.lead_shard[prepare.tid := prepare.lead_participant]))]);
-                    var this_1 := this_2.(network := this_2.network.send(dst, Event.eClockTimeReq(tClockTimeReq.New(dst, prepare.tid)), this_2.machines[dst].shard.localClock));
-                    this_1;
+    var this_4 :=
+      if
+        prepare.tid in this_5.machines[dst].shard.aborted
+      then
+        var this_0 :=
+          this_5.(network :=
+          this_5.network.send(dst, Event.eShardPrepareRsp(tShardPrepareRsp.New(dst, prepare.tid, tShardPrepareStatus.SHARD_ABORT(), INVALID_TIME())), prepare.router));
+        this_0
+      else
+        var this_3 :=
+          this_5.(machines :=
+          this_5.machines[dst :=
+          this_5.machines[dst].(shard :=
+          this_5.machines[dst].shard.(router :=
+          this_5.machines[dst].shard.router[prepare.tid :=
+          prepare.router]))]);
+        var this_2 :=
+          this_3.(machines :=
+          this_3.machines[dst :=
+          this_3.machines[dst].(shard :=
+          this_3.machines[dst].shard.(lead_shard :=
+          this_3.machines[dst].shard.lead_shard[prepare.tid :=
+          prepare.lead_participant]))]);
+        var this_1 :=
+          this_2.(network :=
+          this_2.network.send(dst, Event.eClockTimeReq(tClockTimeReq.New(dst, prepare.tid)), this_2.machines[dst].shard.localClock));
+        this_1;
 
     this_4
   }
 
-  function deliver_eClockTimeRsp_to_Shard_in_WaitForRequests(src: MachineID, dst: MachineID, payload: tClockTimeRsp): System
+  function deliver_eClockTimeRsp_to_Shard_in_EventLoop(src: MachineID, dst: MachineID, payload: tClockTimeRsp): System
     requires src in machines
     requires dst in machines
     requires network.receivable(src, dst)
     requires network.receive(src, dst).0.eClockTimeRsp?
     requires network.receive(src, dst).0.TClockTimeRsp == payload
     requires machines[dst].Shard?
-    requires machines[dst].shard.state.WaitForRequests?
+    requires machines[dst].shard.state.EventLoop?
   {
-    var (event, network') := network.receive(src, dst);
+    var (event, network') :=
+      network.receive(src, dst);
 
-    var this_2 := this.(network := network');
+    var this_4 :=
+      this.(network :=
+      network');
 
-    var this_1 := this_2.(machines := this_2.machines[dst := this_2.machines[dst].(shard := this_2.machines[dst].shard.(prepared := this_2.machines[dst].shard.prepared[payload.requestId := max_time(this_2.machines[dst].shard.clock, payload.now.latest)]))]);
+    var tid: tTid :=
+      payload.requestId;
 
-    var this_0 := this_1.(network := this_1.network.send(dst, Event.eShardPrepareRsp(tShardPrepareRsp.New(dst, payload.requestId, tShardPrepareStatus.SHARD_OK(), max_time(this_1.machines[dst].shard.clock, payload.now.latest))), this_1.machines[dst].shard.router[payload.requestId]));
+    var time: tTime :=
+      max_time(this_4.machines[dst].shard.clock, payload.now.latest);
 
-    this_0
+    var this_3 :=
+      if
+        tid in this_4.machines[dst].shard.router
+      then
+        var this_1 :=
+          this_4.(machines :=
+          this_4.machines[dst :=
+          this_4.machines[dst].(shard :=
+          this_4.machines[dst].shard.(prepared :=
+          this_4.machines[dst].shard.prepared[tid :=
+          time]))]);
+        var this_0 :=
+          this_1.(network :=
+          this_1.network.send(dst, Event.eShardPrepareRsp(tShardPrepareRsp.New(dst, tid, tShardPrepareStatus.SHARD_OK(), time)), this_1.machines[dst].shard.router[tid]));
+        this_0
+      else
+        var this_2 :=
+          this_4.(machines :=
+          this_4.machines[dst :=
+          this_4.machines[dst].(shard :=
+          this_4.machines[dst].shard.(state :=
+          ShardState.Error(true)))]);
+        this_2;
+
+    this_3
   }
 
-  function deliver_eShardCommit_to_Shard_in_WaitForRequests(src: MachineID, dst: MachineID, commit: tShardCommit): System
+  function deliver_eShardCommit_to_Shard_in_EventLoop(src: MachineID, dst: MachineID, commit: tShardCommit): System
     requires src in machines
     requires dst in machines
     requires network.receivable(src, dst)
     requires network.receive(src, dst).0.eShardCommit?
     requires network.receive(src, dst).0.TShardCommit == commit
     requires machines[dst].Shard?
-    requires machines[dst].shard.state.WaitForRequests?
+    requires machines[dst].shard.state.EventLoop?
   {
-    var (event, network') := network.receive(src, dst);
+    var (event, network') :=
+      network.receive(src, dst);
 
-    var this_8 := this.(network := network');
+    var this_9 :=
+      this.(network :=
+      network');
 
-    var this_7 := if commit.tid in this_8.machines[dst].shard.write_buff then
-                    var this_6 := this_8.(machines := this_8.machines[dst := this_8.machines[dst].(shard := this_8.machines[dst].shard.(versions := map key: tKey | key in this_8.machines[dst].shard.write_buff[commit.tid] && true :: key := this_8.machines[dst].shard.versions[key][commit.commit_time := this_8.machines[dst].shard.write_buff[commit.tid][key]]))]);
-                    var this_5 := this_6.(machines := this_6.machines[dst := this_6.machines[dst].(shard := this_6.machines[dst].shard.(locked_keys := this_6.machines[dst].shard.locked_keys - set key: tKey | key in this_6.machines[dst].shard.write_buff[commit.tid] && true :: key))]);
-                    var this_4 := this_5.(machines := this_5.machines[dst := this_5.machines[dst].(shard := this_5.machines[dst].shard.(write_buff := this_5.machines[dst].shard.write_buff - {commit.tid}))]);
-                    this_4 else
-                    this_8;
+    var empty: map<tTime, tVal> :=
+      map[];
 
-    var this_3 := if commit.tid in this_7.machines[dst].shard.prepared then
-                    var this_2 := this_7.(machines := this_7.machines[dst := this_7.machines[dst].(shard := this_7.machines[dst].shard.(prepared := this_7.machines[dst].shard.prepared - {commit.tid}))]);
-                    this_2 else
-                    this_7;
+    var this_8 :=
+      if
+        commit.tid in this_9.machines[dst].shard.write_buff
+      then
+        var this_7 :=
+          this_9.(machines :=
+          this_9.machines[dst :=
+          this_9.machines[dst].(shard :=
+          this_9.machines[dst].shard.(versions :=
+          map key: tKey | key in this_9.machines[dst].shard.write_buff[commit.tid] :: key :=
+                                                                                   if
+                                                                                     true && !(key in this_9.machines[dst].shard.versions)
+                                                                                   then
+                                                                                     empty
+                                                                                   else
+                                                                                     this_9.machines[dst].shard.versions[key]))]);
+        var this_6 :=
+          this_7.(machines :=
+          this_7.machines[dst :=
+          this_7.machines[dst].(shard :=
+          this_7.machines[dst].shard.(versions :=
+          map key: tKey | key in this_7.machines[dst].shard.write_buff[commit.tid] :: key :=
+                                                                                   if
+                                                                                     true
+                                                                                   then
+                                                                                     this_7.machines[dst].shard.versions[key][commit.commit_time :=
+                                                                                     this_7.machines[dst].shard.write_buff[commit.tid][key]]
+                                                                                   else
+                                                                                     this_7.machines[dst].shard.versions[key]))]);
+        var this_5 :=
+          this_6.(machines :=
+          this_6.machines[dst :=
+          this_6.machines[dst].(shard :=
+          this_6.machines[dst].shard.(locked_keys :=
+          this_6.machines[dst].shard.locked_keys - set key: tKey | key in this_6.machines[dst].shard.write_buff[commit.tid] && true :: key))]);
+        var this_4 :=
+          this_5.(machines :=
+          this_5.machines[dst :=
+          this_5.machines[dst].(shard :=
+          this_5.machines[dst].shard.(write_buff :=
+          this_5.machines[dst].shard.write_buff - {commit.tid}))]);
+        this_4
+      else
+        this_9;
 
-    var this_1 := this_3.(machines := this_3.machines[dst := this_3.machines[dst].(shard := this_3.machines[dst].shard.(committed := this_3.machines[dst].shard.committed[commit.tid := commit.commit_time]))]);
+    var this_3 :=
+      if
+        commit.tid in this_8.machines[dst].shard.prepared
+      then
+        var this_2 :=
+          this_8.(machines :=
+          this_8.machines[dst :=
+          this_8.machines[dst].(shard :=
+          this_8.machines[dst].shard.(prepared :=
+          this_8.machines[dst].shard.prepared - {commit.tid}))]);
+        this_2
+      else
+        this_8;
 
-    var this_0 := this_1.(machines := this_1.machines[dst := this_1.machines[dst].(shard := this_1.machines[dst].shard.(pending_reads := map read: tShardReadReq | read in this_1.machines[dst].shard.pending_reads && true && commit.tid in this_1.machines[dst].shard.pending_reads[read] :: read := this_1.machines[dst].shard.pending_reads[read] - {commit.tid}))]);
+    var this_1 :=
+      this_3.(machines :=
+      this_3.machines[dst :=
+      this_3.machines[dst].(shard :=
+      this_3.machines[dst].shard.(committed :=
+      this_3.machines[dst].shard.committed[commit.tid :=
+      commit.commit_time]))]);
+
+    var this_0 :=
+      this_1.(machines :=
+      this_1.machines[dst :=
+      this_1.machines[dst].(shard :=
+      this_1.machines[dst].shard.(pending_reads :=
+      map read: tShardReadReq | read in this_1.machines[dst].shard.pending_reads :: read :=
+                                                                                 if
+                                                                                   true && commit.tid in this_1.machines[dst].shard.pending_reads[read]
+                                                                                 then
+                                                                                   this_1.machines[dst].shard.pending_reads[read] - {commit.tid}
+                                                                                 else
+                                                                                   this_1.machines[dst].shard.pending_reads[read]))]);
 
     this_0
   }
 
-  function deliver_eShardAbort_to_Shard_in_WaitForRequests(src: MachineID, dst: MachineID, abort: tShardAbort): System
+  function deliver_eShardAbort_to_Shard_in_EventLoop(src: MachineID, dst: MachineID, abort: tShardAbort): System
     requires src in machines
     requires dst in machines
     requires network.receivable(src, dst)
     requires network.receive(src, dst).0.eShardAbort?
     requires network.receive(src, dst).0.TShardAbort == abort
     requires machines[dst].Shard?
-    requires machines[dst].shard.state.WaitForRequests?
+    requires machines[dst].shard.state.EventLoop?
   {
-    var (event, network') := network.receive(src, dst);
+    var (event, network') :=
+      network.receive(src, dst);
 
-    var this_7 := this.(network := network');
+    var this_7 :=
+      this.(network :=
+      network');
 
-    var this_6 := if abort.tid in this_7.machines[dst].shard.write_buff then
-                    var this_5 := this_7.(machines := this_7.machines[dst := this_7.machines[dst].(shard := this_7.machines[dst].shard.(locked_keys := this_7.machines[dst].shard.locked_keys - set key: tKey | key in this_7.machines[dst].shard.write_buff[abort.tid] && true :: key))]);
-                    var this_4 := this_5.(machines := this_5.machines[dst := this_5.machines[dst].(shard := this_5.machines[dst].shard.(write_buff := this_5.machines[dst].shard.write_buff - {abort.tid}))]);
-                    this_4 else
-                    this_7;
+    var this_6 :=
+      if
+        abort.tid in this_7.machines[dst].shard.write_buff
+      then
+        var this_5 :=
+          this_7.(machines :=
+          this_7.machines[dst :=
+          this_7.machines[dst].(shard :=
+          this_7.machines[dst].shard.(locked_keys :=
+          this_7.machines[dst].shard.locked_keys - set key: tKey | key in this_7.machines[dst].shard.write_buff[abort.tid] && true :: key))]);
+        var this_4 :=
+          this_5.(machines :=
+          this_5.machines[dst :=
+          this_5.machines[dst].(shard :=
+          this_5.machines[dst].shard.(write_buff :=
+          this_5.machines[dst].shard.write_buff - {abort.tid}))]);
+        this_4
+      else
+        this_7;
 
-    var this_3 := if abort.tid in this_6.machines[dst].shard.prepared then
-                    var this_2 := this_6.(machines := this_6.machines[dst := this_6.machines[dst].(shard := this_6.machines[dst].shard.(prepared := this_6.machines[dst].shard.prepared - {abort.tid}))]);
-                    this_2 else
-                    this_6;
+    var this_3 :=
+      if
+        abort.tid in this_6.machines[dst].shard.prepared
+      then
+        var this_2 :=
+          this_6.(machines :=
+          this_6.machines[dst :=
+          this_6.machines[dst].(shard :=
+          this_6.machines[dst].shard.(prepared :=
+          this_6.machines[dst].shard.prepared - {abort.tid}))]);
+        this_2
+      else
+        this_6;
 
-    var this_1 := this_3.(machines := this_3.machines[dst := this_3.machines[dst].(shard := this_3.machines[dst].shard.(aborted := this_3.machines[dst].shard.aborted + {abort.tid}))]);
+    var this_1 :=
+      this_3.(machines :=
+      this_3.machines[dst :=
+      this_3.machines[dst].(shard :=
+      this_3.machines[dst].shard.(aborted :=
+      this_3.machines[dst].shard.aborted + {abort.tid}))]);
 
-    var this_0 := this_1.(machines := this_1.machines[dst := this_1.machines[dst].(shard := this_1.machines[dst].shard.(pending_reads := map read: tShardReadReq | read in this_1.machines[dst].shard.pending_reads && true && abort.tid in this_1.machines[dst].shard.pending_reads[read] :: read := this_1.machines[dst].shard.pending_reads[read] - {abort.tid}))]);
+    var this_0 :=
+      this_1.(machines :=
+      this_1.machines[dst :=
+      this_1.machines[dst].(shard :=
+      this_1.machines[dst].shard.(pending_reads :=
+      map read: tShardReadReq | read in this_1.machines[dst].shard.pending_reads :: read :=
+                                                                                 if
+                                                                                   true && abort.tid in this_1.machines[dst].shard.pending_reads[read]
+                                                                                 then
+                                                                                   this_1.machines[dst].shard.pending_reads[read] - {abort.tid}
+                                                                                 else
+                                                                                   this_1.machines[dst].shard.pending_reads[read]))]);
 
     this_0
   }
 
-  function deliver_eShardCommitReq_to_Shard_in_WaitForRequests(src: MachineID, dst: MachineID, commit: tShardCommitReq): System
+  function deliver_eShardCommitReq_to_Shard_in_EventLoop(src: MachineID, dst: MachineID, commit: tShardCommitReq): System
     requires src in machines
     requires dst in machines
     requires network.receivable(src, dst)
     requires network.receive(src, dst).0.eShardCommitReq?
     requires network.receive(src, dst).0.TShardCommitReq == commit
     requires machines[dst].Shard?
-    requires machines[dst].shard.state.WaitForRequests?
+    requires machines[dst].shard.state.EventLoop?
   {
-    var (event, network') := network.receive(src, dst);
+    var (event, network') :=
+      network.receive(src, dst);
 
-    var this_5 := this.(network := network');
+    var this_5 :=
+      this.(network :=
+      network');
 
-    var this_4 := if commit.tid in this_5.machines[dst].shard.aborted then
-                    var this_0 := this_5.(network := this_5.network.send(dst, Event.eShardCommitRsp(tShardCommitRsp.New(dst, commit.tid, tTxnStatus.ABORTED(), INVALID_TIME())), commit.router));
-                    this_0 else
-                    var this_3 := this_5.(machines := this_5.machines[dst := this_5.machines[dst].(shard := this_5.machines[dst].shard.(committed := this_5.machines[dst].shard.committed[commit.tid := max_time(this_5.machines[dst].shard.clock, commit.max_prepare_time)]))]);
-                    var this_2 := this_3.(machines := this_3.machines[dst := this_3.machines[dst].(shard := this_3.machines[dst].shard.(router := this_3.machines[dst].shard.router[commit.tid := commit.router]))]);
-                    var this_1 := this_2.(network := this_2.network.send(dst, Event.eClockAlarmReq(tClockAlarmReq.New(dst, commit.tid, max_time(this_2.machines[dst].shard.clock, commit.max_prepare_time))), this_2.machines[dst].shard.localClock));
-                    this_1;
+    var this_4 :=
+      if
+        commit.tid in this_5.machines[dst].shard.aborted
+      then
+        var this_0 :=
+          this_5.(network :=
+          this_5.network.send(dst, Event.eShardCommitRsp(tShardCommitRsp.New(dst, commit.tid, tTxnStatus.ABORTED(), INVALID_TIME())), commit.router));
+        this_0
+      else
+        var time: tTime :=
+          max_time(this_5.machines[dst].shard.clock, commit.max_prepare_time);
+        var this_3 :=
+          this_5.(machines :=
+          this_5.machines[dst :=
+          this_5.machines[dst].(shard :=
+          this_5.machines[dst].shard.(committed :=
+          this_5.machines[dst].shard.committed[commit.tid :=
+          time]))]);
+        var this_2 :=
+          this_3.(machines :=
+          this_3.machines[dst :=
+          this_3.machines[dst].(shard :=
+          this_3.machines[dst].shard.(router :=
+          this_3.machines[dst].shard.router[commit.tid :=
+          commit.router]))]);
+        var this_1 :=
+          this_2.(network :=
+          this_2.network.send(dst, Event.eClockAlarmReq(tClockAlarmReq.New(dst, commit.tid, time)), this_2.machines[dst].shard.localClock));
+        this_1;
 
     this_4
   }
 
-  function deliver_eClockAlarmRsp_to_Shard_in_WaitForRequests(src: MachineID, dst: MachineID, alarm: tClockAlarmRsp): System
+  function deliver_eClockAlarmRsp_to_Shard_in_EventLoop(src: MachineID, dst: MachineID, alarm: tClockAlarmRsp): System
     requires src in machines
     requires dst in machines
     requires network.receivable(src, dst)
     requires network.receive(src, dst).0.eClockAlarmRsp?
     requires network.receive(src, dst).0.TClockAlarmRsp == alarm
     requires machines[dst].Shard?
-    requires machines[dst].shard.state.WaitForRequests?
+    requires machines[dst].shard.state.EventLoop?
   {
-    var (event, network') := network.receive(src, dst);
+    var (event, network') :=
+      network.receive(src, dst);
 
-    var this_8 := this.(network := network');
+    var this_11 :=
+      this.(network :=
+      network');
 
-    var this_7 := if alarm.requestId in this_8.machines[dst].shard.write_buff then
-                    var this_6 := this_8.(machines := this_8.machines[dst := this_8.machines[dst].(shard := this_8.machines[dst].shard.(versions := map key: tKey | key in this_8.machines[dst].shard.write_buff[alarm.requestId] && true :: key := this_8.machines[dst].shard.versions[key][this_8.machines[dst].shard.committed[alarm.requestId] := this_8.machines[dst].shard.write_buff[alarm.requestId][key]]))]);
-                    var this_5 := this_6.(machines := this_6.machines[dst := this_6.machines[dst].(shard := this_6.machines[dst].shard.(locked_keys := this_6.machines[dst].shard.locked_keys - set key: tKey | key in this_6.machines[dst].shard.write_buff[alarm.requestId] && true :: key))]);
-                    var this_4 := this_5.(machines := this_5.machines[dst := this_5.machines[dst].(shard := this_5.machines[dst].shard.(write_buff := this_5.machines[dst].shard.write_buff - {alarm.requestId}))]);
-                    this_4 else
-                    this_8;
+    var empty: map<tTime, tVal> :=
+      map[];
 
-    var this_3 := if alarm.requestId in this_7.machines[dst].shard.prepared then
-                    var this_2 := this_7.(machines := this_7.machines[dst := this_7.machines[dst].(shard := this_7.machines[dst].shard.(prepared := this_7.machines[dst].shard.prepared - {alarm.requestId}))]);
-                    this_2 else
-                    this_7;
+    var tid: tTid :=
+      alarm.requestId;
 
-    var this_1 := this_3.(machines := this_3.machines[dst := this_3.machines[dst].(shard := this_3.machines[dst].shard.(pending_reads := map read: tShardReadReq | read in this_3.machines[dst].shard.pending_reads && true && alarm.requestId in this_3.machines[dst].shard.pending_reads[read] :: read := this_3.machines[dst].shard.pending_reads[read] - {alarm.requestId}))]);
+    var this_10 :=
+      if
+        tid in this_11.machines[dst].shard.committed && tid in this_11.machines[dst].shard.router
+      then
+        var time: tTime :=
+          this_11.machines[dst].shard.committed[tid];
+        var this_8 :=
+          if
+            tid in this_11.machines[dst].shard.write_buff
+          then
+            var this_7 :=
+              this_11.(machines :=
+              this_11.machines[dst :=
+              this_11.machines[dst].(shard :=
+              this_11.machines[dst].shard.(versions :=
+              map key: tKey | key in this_11.machines[dst].shard.write_buff[tid] :: key :=
+                                                                                 if
+                                                                                   true && !(key in this_11.machines[dst].shard.versions)
+                                                                                 then
+                                                                                   empty
+                                                                                 else
+                                                                                   this_11.machines[dst].shard.versions[key]))]);
+            var this_6 :=
+              this_7.(machines :=
+              this_7.machines[dst :=
+              this_7.machines[dst].(shard :=
+              this_7.machines[dst].shard.(versions :=
+              map key: tKey | key in this_7.machines[dst].shard.write_buff[tid] :: key :=
+                                                                                if
+                                                                                  true
+                                                                                then
+                                                                                  this_7.machines[dst].shard.versions[key][time :=
+                                                                                  this_7.machines[dst].shard.write_buff[tid][key]]
+                                                                                else
+                                                                                  this_7.machines[dst].shard.versions[key]))]);
+            var this_5 :=
+              this_6.(machines :=
+              this_6.machines[dst :=
+              this_6.machines[dst].(shard :=
+              this_6.machines[dst].shard.(locked_keys :=
+              this_6.machines[dst].shard.locked_keys - set key: tKey | key in this_6.machines[dst].shard.write_buff[tid] && true :: key))]);
+            var this_4 :=
+              this_5.(machines :=
+              this_5.machines[dst :=
+              this_5.machines[dst].(shard :=
+              this_5.machines[dst].shard.(write_buff :=
+              this_5.machines[dst].shard.write_buff - {tid}))]);
+            this_4
+          else
+            this_11;
+        var this_3 :=
+          if
+            tid in this_8.machines[dst].shard.prepared
+          then
+            var this_2 :=
+              this_8.(machines :=
+              this_8.machines[dst :=
+              this_8.machines[dst].(shard :=
+              this_8.machines[dst].shard.(prepared :=
+              this_8.machines[dst].shard.prepared - {tid}))]);
+            this_2
+          else
+            this_8;
+        var this_1 :=
+          this_3.(machines :=
+          this_3.machines[dst :=
+          this_3.machines[dst].(shard :=
+          this_3.machines[dst].shard.(pending_reads :=
+          map read: tShardReadReq | read in this_3.machines[dst].shard.pending_reads :: read :=
+                                                                                     if
+                                                                                       true && tid in this_3.machines[dst].shard.pending_reads[read]
+                                                                                     then
+                                                                                       this_3.machines[dst].shard.pending_reads[read] - {tid}
+                                                                                     else
+                                                                                       this_3.machines[dst].shard.pending_reads[read]))]);
+        var this_0 :=
+          this_1.(network :=
+          this_1.network.send(dst, Event.eShardCommitRsp(tShardCommitRsp.New(dst, tid, tTxnStatus.COMMITTED(), this_1.machines[dst].shard.committed[tid])), this_1.machines[dst].shard.router[tid]));
+        this_0
+      else
+        var this_9 :=
+          this_11.(machines :=
+          this_11.machines[dst :=
+          this_11.machines[dst].(shard :=
+          this_11.machines[dst].shard.(state :=
+          ShardState.Error(true)))]);
+        this_9;
 
-    var this_0 := this_1.(network := this_1.network.send(dst, Event.eShardCommitRsp(tShardCommitRsp.New(dst, alarm.requestId, tTxnStatus.COMMITTED(), this_1.machines[dst].shard.committed[alarm.requestId])), this_1.machines[dst].shard.router[alarm.requestId]));
-
-    this_0
+    this_10
   }
 
-  function deliver_eShardInquireReq_to_Shard_in_WaitForRequests(src: MachineID, dst: MachineID, inquire: tShardInquireReq): System
+  function deliver_eShardInquireReq_to_Shard_in_EventLoop(src: MachineID, dst: MachineID, inquire: tShardInquireReq): System
     requires src in machines
     requires dst in machines
     requires network.receivable(src, dst)
     requires network.receive(src, dst).0.eShardInquireReq?
     requires network.receive(src, dst).0.TShardInquireReq == inquire
     requires machines[dst].Shard?
-    requires machines[dst].shard.state.WaitForRequests?
+    requires machines[dst].shard.state.EventLoop?
   {
-    var (event, network') := network.receive(src, dst);
+    var (event, network') :=
+      network.receive(src, dst);
 
-    var this_4 := this.(network := network');
+    var this_4 :=
+      this.(network :=
+      network');
 
-    var this_3 := if inquire.tid in this_4.machines[dst].shard.committed then
-                    var this_0 := this_4.(network := this_4.network.send(dst, Event.eShardInquireRsp(tShardInquireRsp.New(inquire.tid, tTxnStatus.COMMITTED(), this_4.machines[dst].shard.committed[inquire.tid], inquire.read)), inquire.shard));
-                    this_0 else
-                    var this_2 := this_4.(machines := this_4.machines[dst := this_4.machines[dst].(shard := this_4.machines[dst].shard.(clock := max_time(this_4.machines[dst].shard.clock, inquire.read.start_time)))]);
-                    var this_1 := this_2.(network := this_2.network.send(dst, Event.eShardInquireRsp(tShardInquireRsp.New(inquire.tid, tTxnStatus.ACTIVE(), INVALID_TIME(), inquire.read)), inquire.shard));
-                    this_1;
+    var this_3 :=
+      if
+        inquire.tid in this_4.machines[dst].shard.committed
+      then
+        var this_0 :=
+          this_4.(network :=
+          this_4.network.send(dst, Event.eShardInquireRsp(tShardInquireRsp.New(inquire.tid, tTxnStatus.COMMITTED(), this_4.machines[dst].shard.committed[inquire.tid], inquire.read)), inquire.shard));
+        this_0
+      else
+        var this_2 :=
+          this_4.(machines :=
+          this_4.machines[dst :=
+          this_4.machines[dst].(shard :=
+          this_4.machines[dst].shard.(clock :=
+          max_time(this_4.machines[dst].shard.clock, inquire.read.start_time)))]);
+        var this_1 :=
+          this_2.(network :=
+          this_2.network.send(dst, Event.eShardInquireRsp(tShardInquireRsp.New(inquire.tid, tTxnStatus.ACTIVE(), INVALID_TIME(), inquire.read)), inquire.shard));
+        this_1;
 
     this_3
   }
